<?xml version="1.0" encoding="utf-8"?>
<section xml:id="section-2" xmlns:xi="http://www.w3.org/2001/XInclude">
  <title>Fourth Solution</title>
  <p>
  This solution is by induction on the power <m>k</m> with the multiplication 
  algorithm.  This solution will prove that if the base-<m>2n</m> digits of
  <m>n^{k-1}</m> are all at least <m>2(d+1)</m> then the base-<m>2n</m> digits of 
  <m>n^k</m> are all at least <m>d+1</m>.
</p>
<p>
The concept of this solution is simple.  Multiplying <m>n^{k-1} \cdot n</m> using 
the elementary school multiplication algorithmin base <m>2n</m>, if every digit of 
<m>n^{k-1}</m> is at least <m>2d</m>, then every carry is between <m>d</m> and <m>m-1</m>.
Therefore every digit of the product is of the form <m>x + r \mod (2n)</m> where <m>x</m>
is either <m>0</m> or <m>n</m>, that is, <m>n</m> times a digit <m>\mod (2n)</m>, 
and <m>d \le r \le n-1</m>.  In particular, every digit is at least <m>d</m>.  Note that
in particular, it is necessary to recognize that each carry is at most <m>m-1</m>.
If <m>n</m> carried over to an odd digit of <m>n^{k-1}</m>, then the corresponding 
digit of <m>n^{k}</m> would be <m>0</m> which is less than <m>d</m>.
<p>
The base case <m>k=1</m> is true if <m>N = d</m>. That is, for an odd integer <m>n > N</m>
the base-<m>2n</m> representation of <m>n</m> which will be the 
single <lq>digit<rq> <m>n</m> which then satisifies <m>n \gt N = d</m>.
</p>
<p>
<lemma>
    <title>Multiplication</title>
  <statement>
    <p>
      Let the base-<m>2n</m> digits of <m>A</m> be <m>a_{m}a_{m-1} \dots a_{1}a_{0}</m>.
      In other words, <m>0 \le a_i \le 2n</m> and <m>A = \sum_{i=0}^m a_i (2n)^{i}</m>.
      Iteratively define the digits of <m> n \cdot A </m> as <m>c_i</m> with carries <m>r_i</m>
      as <m>r_0 = 0</m>, <m>c_i = \operatorname{rem}(n a_i + r_i, 2n)</m>, 
      and 
      <me>
          r_{i+1} = \left\lfloor \frac{n a_i + r_i}{2n} \right\rfloor
      </me>.
       Then 
       <ol>
       <li> <m>0 \le c_i \le 2n</m> for each <m>i \ge 0</m>.</li>
       <li> <m>0 \le r_i < n</m> for each <m>i \ge 0</m>.</li>
       <li> <m> n \cdot A = \sum_{i=0}^{m+1} c_i (2n)^{i}</m></li>
    </ol>     
    </p>
  </statement>

  <proof>
    <p>
      <ol>
      <li> The first item is true by definition since <m>c_i</m> is a 
      remainder modulo <m>2n</m>. </li>
      <li> Prove the second item by induction on <m>i</m>.  The base case is
      true since <m>r_0=0</m> and then if <m>r_i < n</m>
      <me>
      0 \le r_{i+1} \le \left\lfloor \frac{n(2n-1) + (n-1)}{2n} \right\rfloor = n-1
      <me>,
      establishing the induction step.</li>
      <li>To prove the third item, let <m>s_k = \sum_{i=0}^{k} c_i (2n)^i</m>.  By induction
      on <m>k</m>, <m>s_k \equiv nA \mod (2n)^{k+1}</m>.  Since <m>n \cdot A \lt n \cdot (2n)^{m}</m>
      and <m>0 \le s_{m+1} \lt (2n)^{m+1}</m>, this implies <m>n \cdot A = s_{m+1}</m>, 
      completing the proof.
    </p>
  </proof>
</theorem>

