<?xml version="1.0" encoding="utf-8"?>
<section xml:id="secondsolution" xmlns:xi="http://www.w3.org/2001/XInclude">
  <title>Second Solution</title>
  <p>
  Following the first four paragraphs of the First Solution,
  recall that <m> n^{i+1}</m> divides <m>s_i</m>.  Denote 
  <m>t_i = s_i/n^{i+1}</m>.   
  Recall that the units digit is <m>c_0 = n</m> so 
  <m>s_i \gt 0</m> and therefore <m>t_i \ge 1</m>.  We have
  <me>
  c_i = \left\lfloor \frac{s_i}{(2n)^i} \right\rfloor 
      = \left\lfloor \frac{nt_i}{2^i}\right\rfloor
      \ge \left\lfloor \frac{n}{2^i}\right\rfloor
  </me>. 
  </p>
  <p>
  As noted in the First Solution 
  <m>n^k \lt (2n)^k</m>, so <m>n^k</m> has at most <m>k</m> 
    digits when expressed in base <m>2n</m>.  So we may always assume 
    <m>i \lt  k</m>.  If <m> n \gt 2^{k-1}(d + 1)</m>, then 
    <me>
    c_i \ge  \left\lfloor \frac{n}{2^i}\right\rfloor \ge 
    \left\lfloor \frac{2^{k-1}(d+1)}{2^{k-1}}\right\rfloor 
    = (d+1)
    </me>
    as desired.
  </p>
  <p>
  Another way to prove 
  <me>
   c_i = \left\lfloor \frac{nt_i}{2^i}\right\rfloor
   </me>
   is to first to recall that <m>s_i = t_i \cdot n^{i+1}</m> 
   and <m>s_{i-1} = t_{i-1} \cdot n^i</m>.  Then
   <me>
   c_i = \frac{s_i - s_{i-1}}{(2n)^i} 
   = \frac{n t_i - t_{i-1}}{2^i}
   </me>.
   But <m>s_i \lt (2n)^{i+1}</m>, so <m>t_i \lt 2^{i+1}</m> in general, and for the
   next inequality in particular <m>t_{i-1} \lt 2^i</m>. Then
   <me>  \frac{nt_i - t_{i-1}}{2^i} = \frac{n t_i}{2^i} - \frac{t_{i-1}}{2^i} = 
   \left\lfloor \frac{nt_i}{2^i}\right\rfloor
   </me>. 
Then the proof proceeds as before.
</p>
</section>
