<?xml version="1.0" encoding="utf-8"?>
<section xml:id="section-1" xmlns:xi="http://www.w3.org/2001/XInclude">
  <title>Solutions</title>
  <introduction>
    <p>I use the following notation throughout this article: 
    <ul>
    <li> <m>c_i</m> denotes the digit of 
    <m>n^k</m> in the <m>(2n)^i</m> place, and</li> 
    <li> <m>s_i</m> denotes the base <m>2n</m> number 
    <m>c_{i}c_{i-1}\dots c_{2}c_{1}c_{0}</m> which is the truncation of <m>n^k</m> at the 
    <m>i+1</m> rightmost digits. </li> 
    </ul>
    Note that obviously <m>n^k \lt (2n)^k = 2^k n^k</m>, so <m>n^k</m> has at most <m>k</m> 
    digits in places <m>(2n)^{k-1}</m> down to the units place <m>(2n)^0</m> 
    when expressed in base <m>2n</m>. 
    I find it mathematically clearer to write <m>n^k</m> in base <m>2n</m> as
    <me>
    n^k = c_{k-1}(2n)^{k-1} + c_{k-2}(2n)^{i-2} + \dots + c_1(2n)^1 + c_0(2n)^0
    </me>.  The goal is to
    prove that there is a positive integer <m>N</m> such that for every odd <m>n > N</m> the 
    coefficients satisfy <m>c_i\geq d+1</m> for all <m>i\geq 0</m>.</p> 
  </introduction>
  <subsection xml:id="subsection-1">
    <title>First solution</title>
    <p>Let <m>\operatorname{rem}(x,y)</m> denote the remainder when 
    <m>x</m> is divided by <m>y</m>.  Using the standard notation
    <me>
        c_i = \left\lfloor \frac{n^k}{(2n)^i} \right\rfloor \% (2n) 
            = \left\lfloor \frac{n^{k-i}{2^i} \right\rfloor \% (2n)
    </me>
    The first equality follows because the division by <m>(2n)^i</m> will make the series
    expansion with powers <m>j \lt i</m> less than <m>1</m>, so the floor function truncates them 
    off.  Then remainder by <m>2n</m> operation eliminates all but the constant term <m>c_i</m>.
    The second equality follows by simple division. Now the claim is
    <me>
    \left\lfloor \frac{n^{k-i}}{2^i} \right\rfloor%(2n) = 
    \left\lfloor \frac{n^{k-i}%(2^{i+1}n)}{2^i} \right\rfloor,
    </me>
    that is, it is possible to move the remainder operation inside the floor function with 
    appropriate modification.  
    </p>
  </subsection>

    <subsection xml:id="subsection-2">
        <title>Second solution</title>
    <p>
    Note that obviously <m>n^k \lt (2n)^k</m>, so <m>n^k</m> has at most <m>k</m> 
    digits when expressed in base <m>2n</m> or equivalenty the power sum will have
    at most <m>k</m> terms from power <m>(2n)^{k-1}</m> down to <m>(2n)^0</m>.  
    Note that some of the leading digits or highest power coefficients may be zero.  
    An example is <m>n=5</m> and <m>k=4</m>, where 
    <m>n^k = 5^4 = 625 = 0(2 \cdot 5)^3 + 6(2 \cdot 5)^2 + 2(2 \cdot 5)^1 + 5(2 \cdot 5)^0</m>.
    </p>
    <p>
    The next claim is that <m>n^k \equiv n (\mod (2n)</m>.  The proof is by induction.  The base
    case is <m>k=1</m>, where <m>n^1 \equiv n (\mod (2n)</m> is trivially true.  The inductive step
    starts with <m>n^{k+1} = n^k \cdot n \equiv n \cdot n = n^2 \mod (2n)</m>.  Since <m>n</m> is odd, <m>n = 2m + 1</m>
    for some <m>m</m>.  Then <m>n^2 = (2m+1) \cdot n = (2m)n + n \equiv n (\mod (2n)</m> is also  true.  The inductive step is complete.
    The conclusion drawn from this fact is that the units 
    digit is <m>n</m>.</p>
    <p>
    Keeping with the established notation,<m>c_i</m> denotes the digit of 
    <m>n^k</m> in the <m>(2n)^i</m> place, so in the power sum form
    <me>
    n^k = \sum_{i=0}^{k-1} c_i (2n)^i, 0 \le c_i \lt (2n)
    </me>
    and <m>s_i</m> denotes the base <m>2n</m> number which is the truncation 
    of <m>n^k</m> at the 
    <m>i+1</m>rightmost digits, so
    <me>
    s_i = \sum_{j=0}^{i} \sum_{i=0}^{i} c_j (2n)^j, 0 \le c_j \lt (2n)
    </me>
    for each <m>i</m>.
    </p>
    <p>
    Note that <m>n^k - s_i</m> has only terms of power <m>(2n)^{i+1}</m> and higher.  
    Then <m>(2n)^{i+1}</m> divides <m>n^k - s_i</m>.  That is, <m>n^k - s_i = q \cdot (2n)^{i+1}</m>
    or equivalently <m>s_i = n^k - q \cdot (2n)^{i+1} = n^{i+1}(n^{k-i-1}- q 2^{i+1})</m> 
    for some integer <m>q</m>. That is <m> n^{i+1}</m> divides <m>s_i</m>.  Now <m>c_0 = n</m>
    so <m>s_i \gt 0 </m> and therefore <m>s_i \ge n^{i+1}</m>.    
    </p>
    <p>
    Now if <m>n > (d+1) \cdot 2^{i+1}</m>, then <m>s_i \ge (d+1) \cdot (2n)^{i} > (d+1)</m>.  
    But this means the digit in the <m>(2n)^i</m> place is at least <m>d+1</m>.  
    Since this is true for all <m>i</m> with <m>0 \le i \le k-1</m>, the problem is finished.
    </p>
    <p> In summary, given <m>k</m> and <m>d</m>, take <m>N=(d+1) \cdot 2^{k-1}</m> so that for every odd <m>n > N</m> all the
    digits in the base <m>2n</m> expansion of <m>n^k</m> are greater than <m>d</m>.
    </p>
    <figure>
      <caption>A frog</caption>
      <image source="frog.jpg" width="50%">
        <description>A nice-looking frog with a longish description.</description>
      </image>
    </figure>
    <p>Bar: <m>\foo</m></p>
  </subsection>
</section>
